theories/Factor_Related_Bags.thy
@@ -1,0 +1,332 @@
+theory Factor_Related_Bags
+  imports Factor_Bag_Comparison
+begin
+
+section \<open>Selection through an actual comparison definition\<close>
+
+definition related_selection_here_schema :: "nat \<Rightarrow> nat \<Rightarrow> (nat,nat,nat) factor_schema" where
+  "related_selection_here_schema compare list=data_rule
+    (Pattern_Pair data_x (Pattern_Pair (Pattern_Pair data_y data_z) data_z))
+    {(0,compare,Pattern_Pair data_x data_y),(1,list,data_z)}"
+
+definition related_selection_clauses ::
+  "nat \<Rightarrow> nat \<Rightarrow> nat \<Rightarrow> nat \<Rightarrow> (nat \<times> (nat,nat,nat) factor_schema) set" where
+  "related_selection_clauses data list compare select=
+    {(0,related_selection_here_schema compare list),(1,selection_later_schema data select)}"
+
+definition related_bag_clauses :: "nat \<Rightarrow> nat \<Rightarrow> (nat \<times> (nat,nat,nat) factor_schema) set" where
+  "related_bag_clauses select bag={(0,bag_nil_schema),(1,bag_step_schema select bag)}"
+
+locale related_bags =
+  fixes P :: "(nat,nat,nat,nat) schema_system"
+    and data_site list_site compare_site select_site bag_site :: nat
+  assumes system_formed: "schema_system_formed P"
+    and selection_family: "\<And>c S. ((select_site,c),S)\<in>system_clauses P \<longleftrightarrow>
+      (c,S)\<in>related_selection_clauses data_site list_site compare_site select_site"
+    and bag_family: "\<And>c S. ((bag_site,c),S)\<in>system_clauses P \<longleftrightarrow>
+      (c,S)\<in>related_bag_clauses select_site bag_site"
+    and selection_call: "\<And>t. schema_call_formed P select_site t \<longleftrightarrow> term_formed t"
+    and bag_call: "\<And>t. schema_call_formed P bag_site t \<longleftrightarrow> term_formed t"
+    and data_meaning: "\<And>t. (data_site,t)\<in>positive_meaning P \<longleftrightarrow>
+      term_formed t \<and> self_contained_term t"
+    and list_meaning: "\<And>t. (list_site,t)\<in>positive_meaning P \<longleftrightarrow>
+      (\<exists>xs. t=data_list_term xs \<and> data_elements xs)"
+    and comparison_data: "\<And>x y. (compare_site,Pair_Term x y)\<in>positive_meaning P \<Longrightarrow>
+      term_formed x \<and> self_contained_term x \<and> term_formed y \<and> self_contained_term y"
+begin
+
+abbreviation related where
+  "related x y \<equiv> (compare_site,Pair_Term x y)\<in>positive_meaning P"
+
+lemma rule:
+  assumes clause: "((d,c),S)\<in>system_clauses P"
+    and selected: "d\<in>{select_site,bag_site}"
+    and ordinary: "schema_material_premises S={}"
+    and assignment: "\<forall>a\<in>schema_variables S. term_formed (f a)"
+    and support: "\<forall>s e p. (s,e,p)\<in>schema_premises S \<longrightarrow>
+      (e,evaluate_pattern f p)\<in>positive_meaning P"
+  shows "(d,evaluate_pattern f (schema_conclusion S))\<in>positive_meaning P"
+proof -
+  have sf: "schema_formed S" using clause system_formed by (auto simp: schema_system_formed_def)
+  have tf: "term_formed (evaluate_pattern f (schema_conclusion S))"
+    by (rule evaluate_pattern_formed)
+      (use sf assignment in \<open>auto simp: schema_formed_def schema_variables_def\<close>)
+  have call: "schema_call_formed P d (evaluate_pattern f (schema_conclusion S))"
+    using selected tf by (auto simp: selection_call bag_call)
+  show ?thesis by (rule ordinary_positive_valuation_step[OF clause ordinary assignment call support])
+qed
+
+theorem selection_sound:
+  assumes holds: "(select_site,t)\<in>positive_meaning P"
+  shows "\<exists>x y pre post. t=Pair_Term x
+    (Pair_Term (data_list_term (pre@y#post)) (data_list_term (pre@post))) \<and>
+    data_elements (pre@y#post) \<and> related x y"
+proof -
+  let ?Q="\<lambda>t. \<exists>x y pre post. t=Pair_Term x
+    (Pair_Term (data_list_term (pre@y#post)) (data_list_term (pre@post))) \<and>
+    data_elements (pre@y#post) \<and> related x y"
+  have invariant: "select_site=select_site \<longrightarrow> ?Q t"
+  proof (rule positive_valuation_induct[OF holds, where property="\<lambda>d t. d=select_site \<longrightarrow> ?Q t"])
+    fix d c S f
+    assume clause: "((d,c),S)\<in>system_clauses P"
+      and assignment: "\<forall>a\<in>schema_variables S. term_formed (f a)"
+      and call: "schema_call_formed P d (evaluate_pattern f (schema_conclusion S))"
+      and support: "\<forall>s e p. (s,e,p)\<in>schema_premises S \<longrightarrow>
+        (e,evaluate_pattern f p)\<in>positive_meaning P \<and>
+        (e=select_site \<longrightarrow> ?Q (evaluate_pattern f p))"
+    show "d=select_site \<longrightarrow> ?Q (evaluate_pattern f (schema_conclusion S))"
+    proof
+      assume "d=select_site"
+      then have cases: "S=related_selection_here_schema compare_site list_site \<or>
+        S=selection_later_schema data_site select_site"
+        using clause by (auto simp: selection_family related_selection_clauses_def)
+      then show "?Q (evaluate_pattern f (schema_conclusion S))"
+      proof
+        assume schema: "S=related_selection_here_schema compare_site list_site"
+        have compared: "related (f 0) (f 1)" and list: "(list_site,f 2)\<in>positive_meaning P"
+          using support schema by (auto simp: related_selection_here_schema_def)
+        have head: "term_formed (f 1) \<and> self_contained_term (f 1)"
+          using comparison_data[OF compared] by blast
+        obtain post where tail: "f 2=data_list_term post" "data_elements post"
+          using list by (auto simp: list_meaning)
+        show ?thesis by (intro exI[of _ "f 0"] exI[of _ "f 1"] exI[of _ "[]"] exI[of _ post])
+          (use head tail compared in \<open>simp add: schema related_selection_here_schema_def\<close>)
+      next
+        assume schema: "S=selection_later_schema data_site select_site"
+        have skipped: "term_formed (f 2) \<and> self_contained_term (f 2)"
+          using support schema by (auto simp: selection_later_schema_def data_meaning)
+        obtain y pre post where tail: "f 1=data_list_term (pre@y#post)"
+          "f 3=data_list_term (pre@post)" "data_elements (pre@y#post)" "related (f 0) y"
+          using support[rule_format, of 1 select_site "Pattern_Pair data_x (Pattern_Pair data_y data_w)"] schema
+          by (auto simp: selection_later_schema_def)
+        show ?thesis by (intro exI[of _ "f 0"] exI[of _ y] exI[of _ "f 2#pre"] exI[of _ post])
+          (use skipped tail in \<open>simp add: schema selection_later_schema_def\<close>)
+      qed
+    qed
+  qed
+  show ?thesis using invariant by simp
+qed
+
+theorem selection_complete:
+  assumes "data_elements (pre@y#post)" "related x y"
+  shows "(select_site,Pair_Term x
+    (Pair_Term (data_list_term (pre@y#post)) (data_list_term (pre@post))))\<in>positive_meaning P"
+  using assms
+proof (induction pre)
+  case Nil
+  have head: "term_formed x" using comparison_data[OF Nil.prems(2)] by blast
+  have tail: "(list_site,data_list_term post)\<in>positive_meaning P"
+    using Nil.prems(1) by (auto simp: list_meaning)
+  let ?f="\<lambda>a::nat. if a=0 then x else if a=1 then y else data_list_term post"
+  have result: "(select_site,evaluate_pattern ?f
+      (schema_conclusion (related_selection_here_schema compare_site list_site)))\<in>positive_meaning P"
+    by (rule rule[where c=0])
+      (use Nil.prems head tail in \<open>auto simp: selection_family related_selection_clauses_def
+        related_selection_here_schema_def schema_variables_def data_list_term_formed\<close>)
+  show ?case using result by (simp add: related_selection_here_schema_def)
+next
+  case (Cons z pre)
+  have head: "term_formed x" using comparison_data[OF Cons.prems(2)] by blast
+  have skipped: "(data_site,z)\<in>positive_meaning P"
+    using Cons.prems(1) by (simp add: data_meaning)
+  have tail: "(select_site,Pair_Term x
+    (Pair_Term (data_list_term (pre@y#post)) (data_list_term (pre@post))))\<in>positive_meaning P"
+    using Cons by auto
+  let ?f="\<lambda>a::nat. if a=0 then x else if a=1 then data_list_term (pre@y#post)
+    else if a=2 then z else data_list_term (pre@post)"
+  have result: "(select_site,evaluate_pattern ?f
+      (schema_conclusion (selection_later_schema data_site select_site)))\<in>positive_meaning P"
+    by (rule rule[where c=1])
+      (use Cons.prems head skipped tail in \<open>auto simp: selection_family related_selection_clauses_def
+        selection_later_schema_def schema_variables_def data_list_term_formed\<close>)
+  show ?case using result by (simp add: selection_later_schema_def)
+qed
+
+theorem selection_exact:
+  "(select_site,t)\<in>positive_meaning P \<longleftrightarrow>
+    (\<exists>x y pre post. t=Pair_Term x
+      (Pair_Term (data_list_term (pre@y#post)) (data_list_term (pre@post))) \<and>
+      data_elements (pre@y#post) \<and> related x y)"
+  using selection_sound selection_complete by blast
+
+section \<open>Matching every occurrence through that same definition\<close>
+
+theorem comparison_sound:
+  assumes holds: "(bag_site,t)\<in>positive_meaning P"
+  shows "\<exists>xs ys. t=Pair_Term (data_list_term xs) (data_list_term ys) \<and>
+    data_elements xs \<and> data_elements ys \<and> rel_mset related (mset xs) (mset ys)"
+proof -
+  let ?Q="\<lambda>t. \<exists>xs ys. t=Pair_Term (data_list_term xs) (data_list_term ys) \<and>
+    data_elements xs \<and> data_elements ys \<and> rel_mset related (mset xs) (mset ys)"
+  have invariant: "bag_site=bag_site \<longrightarrow> ?Q t"
+  proof (rule positive_valuation_induct[OF holds, where property="\<lambda>d t. d=bag_site \<longrightarrow> ?Q t"])
+    fix d c S f
+    assume clause: "((d,c),S)\<in>system_clauses P"
+      and assignment: "\<forall>a\<in>schema_variables S. term_formed (f a)"
+      and call: "schema_call_formed P d (evaluate_pattern f (schema_conclusion S))"
+      and support: "\<forall>s e p. (s,e,p)\<in>schema_premises S \<longrightarrow>
+        (e,evaluate_pattern f p)\<in>positive_meaning P \<and>
+        (e=bag_site \<longrightarrow> ?Q (evaluate_pattern f p))"
+    show "d=bag_site \<longrightarrow> ?Q (evaluate_pattern f (schema_conclusion S))"
+    proof
+      assume "d=bag_site"
+      then have cases: "S=bag_nil_schema \<or> S=bag_step_schema select_site bag_site"
+        using clause by (auto simp: bag_family related_bag_clauses_def)
+      then show "?Q (evaluate_pattern f (schema_conclusion S))"
+      proof
+        assume "S=bag_nil_schema"
+        then show ?thesis by (intro exI[of _ "[]"] exI[of _ "[]"]) (simp add: bag_nil_schema_def)
+      next
+        assume schema: "S=bag_step_schema select_site bag_site"
+        have selection: "(select_site,Pair_Term (f 0) (Pair_Term (f 2) (f 3)))\<in>positive_meaning P"
+          using support schema by (auto simp: bag_step_schema_def)
+        obtain y pre post where selected: "f 2=data_list_term (pre@y#post)"
+          "f 3=data_list_term (pre@post)" "data_elements (pre@y#post)" "related (f 0) y"
+          using selection_sound[OF selection] by auto
+        obtain xs zs where compared: "f 1=data_list_term xs" "f 3=data_list_term zs"
+          "data_elements xs" "data_elements zs" "rel_mset related (mset xs) (mset zs)"
+          using support[rule_format, of 1 bag_site "Pattern_Pair data_y data_w"] schema
+          by (auto simp: bag_step_schema_def)
+        have residual: "zs=pre@post" using selected(2) compared(2)
+          by (simp add: data_list_term_injective)
+        have head: "term_formed (f 0) \<and> self_contained_term (f 0)"
+          using comparison_data[OF selected(4)] by blast
+        have matching: "rel_mset related (mset (f 0#xs)) (mset (pre@y#post))"
+          using rel_mset_Plus[OF selected(4) compared(5)] by (simp add: residual)
+        show ?thesis by (intro exI[of _ "f 0#xs"] exI[of _ "pre@y#post"])
+          (use selected compared head matching in \<open>auto simp: schema bag_step_schema_def\<close>)
+      qed
+    qed
+  qed
+  show ?thesis using invariant by simp
+qed
+
+theorem comparison_complete:
+  assumes "data_elements xs" "data_elements ys" "rel_mset related (mset xs) (mset ys)"
+  shows "(bag_site,Pair_Term (data_list_term xs) (data_list_term ys))\<in>positive_meaning P"
+  using assms
+proof (induction xs arbitrary: ys)
+  case Nil
+  have empty: "ys=[]" using Nil.prems by simp
+  have result: "(bag_site,evaluate_pattern (\<lambda>_. Payload_Term []) (schema_conclusion bag_nil_schema))
+    \<in>positive_meaning P"
+    by (rule rule[where c=0])
+      (auto simp: bag_family related_bag_clauses_def bag_nil_schema_def schema_variables_def)
+  show ?case using result empty by (simp add: bag_nil_schema_def)
+next
+  case (Cons x xs)
+  obtain N y where removal: "mset ys=add_mset y N" "related x y" "rel_mset related (mset xs) N"
+    using msed_rel_invL[OF Cons.prems(3)[simplified]] by blast
+  have inside: "y\<in>set ys"
+  proof -
+    have "y\<in>#mset ys" using removal(1) by simp
+    then show ?thesis by simp
+  qed
+  obtain pre post where split: "ys=pre@y#post" using split_list[OF inside] by blast
+  have residual: "N=mset (pre@post)" using removal(1) by (simp add: split)
+  have data: "data_elements (pre@y#post)" using Cons.prems(2) split by simp
+  have selection: "(select_site,Pair_Term x
+    (Pair_Term (data_list_term ys) (data_list_term (pre@post))))\<in>positive_meaning P"
+    using selection_complete[OF data removal(2)] split by simp
+  have tail: "(bag_site,Pair_Term (data_list_term xs) (data_list_term (pre@post)))\<in>positive_meaning P"
+    by (rule Cons.IH) (use Cons.prems(1) data removal(3) residual in auto)
+  let ?f="\<lambda>a::nat. if a=0 then x else if a=1 then data_list_term xs
+    else if a=2 then data_list_term ys else data_list_term (pre@post)"
+  have result: "(bag_site,evaluate_pattern ?f (schema_conclusion (bag_step_schema select_site bag_site)))
+    \<in>positive_meaning P"
+    by (rule rule[where c=1])
+      (use Cons.prems(1,2) data selection tail in \<open>auto simp: bag_family related_bag_clauses_def
+        bag_step_schema_def schema_variables_def data_list_term_formed\<close>)
+  show ?case using result by (simp add: bag_step_schema_def)
+qed
+
+theorem comparison_exact:
+  "(bag_site,t)\<in>positive_meaning P \<longleftrightarrow>
+    (\<exists>xs ys. t=Pair_Term (data_list_term xs) (data_list_term ys) \<and>
+      data_elements xs \<and> data_elements ys \<and> rel_mset related (mset xs) (mset ys))"
+  using comparison_sound comparison_complete by blast
+
+corollary comparison_lists:
+  "(bag_site,Pair_Term (data_list_term xs) (data_list_term ys))\<in>positive_meaning P \<longleftrightarrow>
+    data_elements xs \<and> data_elements ys \<and> rel_mset related (mset xs) (mset ys)"
+  by (auto simp: comparison_exact data_list_term_injective)
+
+section \<open>Complete collection presentations recover equality of their subjects\<close>
+
+theorem comparison_collections:
+  assumes left: "data_collection_presents read A a"
+    and right: "data_collection_presents read B b"
+    and compare: "\<And>z w x y. read z x \<Longrightarrow> read w y \<Longrightarrow> related x y \<longleftrightarrow> z=w"
+  shows "(bag_site,Pair_Term a b)\<in>positive_meaning P \<longleftrightarrow> A=B"
+proof -
+  have unique: "z=w" if "read z x" "read w x" for z w x
+  proof -
+    have "related x x" using compare[OF that(1) that(1)] by simp
+    then show ?thesis using compare[OF that(1,2)] by blast
+  qed
+  let ?D="\<lambda>x. SOME z. read z x"
+  have decode: "?D x=z" if "read z x" for z x
+    by (rule some_equality[where P="\<lambda>w. read w x", OF that]) (use unique that in blast)
+  have lists: "map ?D ts=xs \<and> (\<forall>x\<in>set ts. read (?D x) x)"
+    if "list_all2 read xs ts" for xs ts
+    using that
+  proof (induction xs arbitrary: ts)
+    case Nil
+    then show ?case by simp
+  next
+    case (Cons z xs)
+    obtain x us where shape: "ts=x#us" and head: "read z x" and tail: "list_all2 read xs us"
+      using Cons.prems by (auto simp: list_all2_Cons1)
+    have decoded: "?D x=z" by (rule decode[OF head])
+    show ?case using Cons.IH[OF tail] head decoded shape by simp
+  qed
+  have formed: "term_formed x \<and> self_contained_term x" if "read z x" for z x
+  proof -
+    have "related x x" using compare[OF that that] by simp
+    then show ?thesis using comparison_data by blast
+  qed
+  obtain xs ts where first: "distinct xs" "set xs=A" "list_all2 read xs ts" "a=data_list_term ts"
+    using left unfolding data_collection_presents_def by blast
+  obtain ys us where second: "distinct ys" "set ys=B" "list_all2 read ys us" "b=data_list_term us"
+    using right unfolding data_collection_presents_def by blast
+  have decoded: "map ?D ts=xs" "map ?D us=ys"
+    and readings: "\<forall>x\<in>set ts. read (?D x) x" "\<forall>y\<in>set us. read (?D y) y"
+    using lists[OF first(3)] lists[OF second(3)] by auto
+  have data: "data_elements ts" "data_elements us" using readings formed by blast+
+  have agreement: "rel_mset related (mset ts) (mset us) =
+    rel_mset (\<lambda>x y. ?D x=?D y) (mset ts) (mset us)"
+    by (rule multiset.rel_cong[OF refl refl])
+      (use readings compare in auto)
+  have mapped: "rel_mset (=) (image_mset ?D (mset ts)) (image_mset ?D (mset us)) =
+    rel_mset (\<lambda>x y. ?D x=?D y) (mset ts) (mset us)"
+    by (simp only: multiset.rel_map)
+  have matching: "rel_mset related (mset ts) (mset us) \<longleftrightarrow> mset xs=mset ys"
+    using agreement mapped by (simp only: multiset.rel_eq mset_map[symmetric] decoded)
+  have identity: "mset xs=mset ys \<longleftrightarrow> A=B"
+    using set_eq_iff_mset_eq_distinct[OF first(1) second(1)] first(2) second(2) by blast
+  show ?thesis using data by (simp add: first(4) second(4) comparison_lists matching identity)
+qed
+
+end
+
+text \<open>
+  The two clause families call explicit definition coordinates in an actual
+  formed program. The relation in the exact comparison theorem is the positive
+  meaning of that program's comparison call. No external predicate enters the
+  operator. The proof permits that definition to participate in the same
+  positive dependency cycle, provided the stated data boundary is established.
+
+  Selection compares two entries, removes precisely the selected occurrence,
+  and checks every skipped entry and the complete retained tail. Each recursive
+  bag step has two distinct premise sockets. Its existential residual is an
+  ordinary fully formed argument at both calls. The resulting relation matches
+  every occurrence through the fixed comparison definition.
+
+  When that callee compares presentations of one subject exactly, the lifted
+  rule compares complete finite collection presentations exactly. Every source
+  entry remains present once, every child presentation may vary, and every
+  enumeration order is admitted. The mathematical decoder used in that proof
+  is a local witness; it is absent from the program and its semantic operator.
+\<close>
+
+end
